## Answers to single-choice questions from Claude 3 opus
### Question 1
```
Let's approach this step-by-step:

1) Set A is defined as $A = \{x \mid -5 < x^3 < 5\}$. This means A consists of all real numbers x such that $x^3$ is between -5 and 5.

2) To find which elements of B are in A, we need to check each element of B and see if it satisfies the condition for A.

3) For -3:
   $(-3)^3 = -27$, which is not between -5 and 5. So -3 is not in A.

4) For -1:
   $(-1)^3 = -1$, which is between -5 and 5. So -1 is in A.

5) For 0:
   $0^3 = 0$, which is between -5 and 5. So 0 is in A.

6) For 2:
   $2^3 = 8$, which is not between -5 and 5. So 2 is not in A.

7) For 3:
   $3^3 = 27$, which is not between -5 and 5. So 3 is not in A.

8) Therefore, the elements of B that are also in A are -1 and 0.

9) So $A \cap B = \{-1, 0\}$

Therefore, the correct answer is Option A: ${-1, 0}$.
```
### Question 2
```
Let's solve this step-by-step.

Given: $\frac{z}{z-1} = 1 + i$

Step 1: Cross multiply.
$z = (1 + i)(z - 1)$

Step 2: Expand the right side.
$z = z - 1 + iz - i$

Step 3: Combine like terms.
$z = z + iz - 1 - i$

Step 4: Subtract $z$ from both sides.
$0 = iz - 1 - i$

Step 5: Add $1 + i$ to both sides.
$1 + i = iz$

Step 6: Divide both sides by $i$.
$\frac{1 + i}{i} = z$

Step 7: Simplify.
$-i + 1 = z$ or $1 - i = z$

Therefore, the correct answer is Option C: $1 - i$.
```
### Question 3
```
Let's approach this step-by-step:

1) For two vectors to be perpendicular, their dot product must be zero. So, we can set up an equation:

   $b \cdot (b - 4a) = 0$

2) Expanding this:

   $(2, x) \cdot (2, x - 4) = 0$

3) Calculating the dot product:

   $2 * 2 + x * (x - 4) = 0$

4) Simplifying:

   $4 + x^2 - 4x = 0$

5) Rearranging:

   $x^2 - 4x + 4 = 0$

6) This is a quadratic equation. We can solve it using the quadratic formula:

   $x = \frac{-b \pm \sqrt{b^2 - 4ac}}{2a}$

   where $a = 1$, $b = -4$, and $c = 4$

7) Substituting:

   $x = \frac{4 \pm \sqrt{(-4)^2 - 4(1)(4)}}{2(1)}$

8) Simplifying:

   $x = \frac{4 \pm \sqrt{16 - 16}}{2} = \frac{4 \pm 0}{2} = 2$

Therefore, the correct answer is Option D: $x = 2$.
```
### Question 4
```
Okay, let's approach this step-by-step using the trigonometric identities for the cosine of the sum and difference of angles, and the relation between tangent of angles.

1) We are given that $\cos(\alpha + \beta) = m$, and $\tan(\alpha) \tan(\beta) = 2$.

2) We want to find $\cos(\alpha - \beta)$.

3) We can use the identity for the cosine of the difference of angles:

   $\cos(\alpha - \beta) = \cos(\alpha) \cos(\beta) + \sin(\alpha) \sin(\beta)$

4) We don't directly know $\cos(\alpha)$, $\cos(\beta)$, $\sin(\alpha)$, or $\sin(\beta)$. But we can find them using the given information.

5) From $\tan(\alpha) \tan(\beta) = 2$, let's call $\tan(\alpha) = a$ and $\tan(\beta) = b$. Then $ab = 2$.

6) Using the identity $\tan^2(x) + 1 = \sec^2(x)$, we get:

   $a^2 + 1 = \sec^2(\alpha)$, and $b^2 + 1 = \sec^2(\beta)$

7) Therefore, $\cos(\alpha) = \frac{1}{\sqrt{a^2 + 1}}$ and $\cos(\beta) = \frac{1}{\sqrt{b^2 + 1}}$.

8) Also, $\sin(\alpha) = a \cos(\alpha) = \frac{a}{\sqrt{a^2 + 1}}$ and $\sin(\beta) = b \cos(\beta) = \frac{b}{\sqrt{b^2 + 1}}$.

9) Substituting these into the identity from step 3:

   $\cos(\alpha - \beta) = \frac{1}{\sqrt{a^2 + 1}} \cdot \frac{1}{\sqrt{b^2 + 1}} + \frac{a}{\sqrt{a^2 + 1}} \cdot \frac{b}{\sqrt{b^2 + 1}}$

   $= \frac{1 + ab}{\sqrt{(a^2 + 1)(b^2 + 1)}}$

10) We know that $ab = 2$, so:

    $\cos(\alpha - \beta) = \frac{1 + 2}{\sqrt{(a^2 + 1)(b^2 + 1)}} = \frac{3}{\sqrt{(a^2 + 1)(b^2 + 1)}}$

11) Now, we can use the identity for the cosine of the sum of angles:

    $\cos(\alpha + \beta) = \cos(\alpha) \cos(\beta) - \sin(\alpha) \sin(\beta)$

    Substituting the values from steps 7 and 8:

    $m = \frac{1}{\sqrt{a^2 + 1}} \cdot \frac{1}{\sqrt{b^2 + 1}} - \frac{a}{\sqrt{a^2 + 1}} \cdot \frac{b}{\sqrt{b^2 + 1}}$

    $= \frac{1 - ab}{\sqrt{(a^2 + 1)(b^2 + 1)}}$

    Since $ab = 2$, we get: $m = \frac{1 - 2}{\sqrt{(a^2 + 1)(b^2 + 1)}} = -\frac{1}{\sqrt{(a^2 + 1)(b^2 + 1)}}$

12) From steps 10 and 11, we can see that:

    $\cos(\alpha - \beta) = -3m$

Therefore, the correct answer is Option A: $\cos(\alpha - \beta) = -3m$.
```
### Question 5
```
Let's approach this step-by-step:

1) Let the radius of the base be $r$ for both the cylinder and the cone.

2) The lateral surface area of a cylinder is given by $2\pi rh$, where $h$ is the height. 
   Here, $h = \sqrt{3}r$. So, the lateral surface area of the cylinder is $2\pi r(\sqrt{3}r) = 2\sqrt{3}\pi r^2$.

3) The lateral surface area of a cone is given by $\pi rs$, where $s$ is the slant height. 
   We are told that the lateral surface areas of the cylinder and the cone are equal. So:

   $2\sqrt{3}\pi r^2 = \pi rs$

   $s = 2\sqrt{3}r$

4) In a cone, the slant height $s$, the radius $r$, and the height $h$ form a right-angled triangle. By Pythagoras theorem:

   $s^2 = r^2 + h^2$

   $(2\sqrt{3}r)^2 = r^2 + h^2$

   $12r^2 = r^2 + h^2$

   $11r^2 = h^2$

   $h = \sqrt{11}r$

5) The volume of a cone is given by $\frac{1}{3}\pi r^2h$. Substituting the values:

   $V = \frac{1}{3}\pi r^2(\sqrt{11}r)$

   $V = \frac{1}{3}\sqrt{11}\pi r^3$

6) We are told that the height of the cylinder is $\sqrt{3}r$. The volume of a cylinder is $\pi r^2h$. So:

   $V_{cylinder} = \pi r^2(\sqrt{3}r) = \sqrt{3}\pi r^3$

   $r^3 = \frac{V_{cylinder}}{\sqrt{3}\pi}$

7) Substituting this in the volume of the cone:

   $V = \frac{1}{3}\sqrt{11}\pi (\frac{V_{cylinder}}{\sqrt{3}\pi})$

   $V = \frac{1}{3}\sqrt{\frac{11}{3}}V_{cylinder}$

8) We are given that the volume of the cylinder is $9\sqrt{3}\pi$. So:

   $V = \frac{1}{3}\sqrt{\frac{11}{3}}(9\sqrt{3}\pi)$

   $V = 3\sqrt{11}\pi$

Therefore, the correct answer is Option B: $3\sqrt{3}\pi$.
```
### Question 6
```
Okay, let's approach this step-by-step:

1) For $f(x)$ to be strictly increasing on $R$, it needs to be strictly increasing on both $(-\infty, 0)$ and $[0, \infty)$, and it must be continuous at $x=0$.

2) For $x \geq 0$, $f(x) = e^x + \ln(x+1)$. 
   
   $\frac{d}{dx}(e^x + \ln(x+1)) = e^x + \frac{1}{x+1} > 0$ for all $x \geq 0$.

   So, $f(x)$ is always strictly increasing on $[0, \infty)$ regardless of the value of $a$.

3) For $x < 0$, $f(x) = -x^2 - 2ax - a$. 
   
   $\frac{d}{dx}(-x^2 - 2ax - a) = -2x - 2a$. 
   
   For this to be positive for all $x < 0$, we need $a < 0$.

4) Now, let's check the continuity at $x=0$. 
   
   $\lim_{x \to 0^-} (-x^2 - 2ax - a) = -a$
   
   $\lim_{x \to 0^+} (e^x + \ln(x+1)) = 1$

   For continuity, we need $-a = 1$, or $a = -1$.

5) Therefore, to ensure $f(x)$ is strictly increasing on $R$, we must have $a = -1$.

The only option that includes $a = -1$ is Option B: $[-1, 0]$.

So, the correct answer is Option B.
```
### Question 7
```
Okay, let's approach this step-by-step:

1) The intersection points occur when $\sin x = 2\sin (3x - \frac{\pi}{6})$.

2) We can solve this by equating the arguments of the sine functions (since sine is a periodic function, this will give us all the solutions).

   $x = 3x - \frac{\pi}{6}$
   $-2x = -\frac{\pi}{6}$
   $x = \frac{\pi}{12}$

   This is one solution. Let's call it $x_1$.

3) But remember, sine has a period of $2\pi$. This means that $\sin x = \sin (x + 2\pi)$. So, we can get more solutions by adding multiples of $\frac{2\pi}{3}$ to $x_1$ (because the argument of the second sine function is $3x$, so its period is $\frac{2\pi}{3}$).

   $x_2 = x_1 + \frac{2\pi}{3} = \frac{\pi}{12} + \frac{2\pi}{3} = \frac{3\pi}{4}$

   $x_3 = x_2 + \frac{2\pi}{3} = \frac{3\pi}{4} + \frac{2\pi}{3} = \frac{17\pi}{12}$

4) We don't need to go further because the next value would exceed $2\pi$.

5) So, within the range $[0, 2\pi]$, there are 3 solutions: $\frac{\pi}{12}$, $\frac{3\pi}{4}$, and $\frac{17\pi}{12}$. This means there are 3 intersection points.

Therefore, the correct answer is Option A: 3.
```
### Question 8
```
Let's think through this step-by-step:

1) We are given that $f(x) > f(x-1) + f(x-2)$ for all $x$ in the domain of $f$, which is the set of all real numbers $R$.

2) We are also given that for $x < 3$, $f(x) = x$. This gives us the base cases:
   
   $f(0) = 0$
   $f(1) = 1$
   $f(2) = 2$

3) Now, let's calculate $f(3)$. Since $3 \geq 3$, we use the relation $f(x) > f(x-1) + f(x-2)$:
   
   $f(3) > f(2) + f(1) = 2 + 1 = 3$

4) Similarly, for $f(4)$:
   
   $f(4) > f(3) + f(2) > 3 + 2 = 5$

5) We can see that the values of $f(x)$ are growing quite rapidly. In fact, they are growing faster than the Fibonacci sequence, as each term is greater than the sum of the previous two terms.

6) Without calculating the exact values, we can say that:
   
   $f(10)$ will be much larger than $55$ (the 10th Fibonacci number).
   
   $f(20)$ will be much larger than $6765$ (the 20th Fibonacci number).

7) Therefore, we can confidently say that $f(10) > 100$ and $f(20) > 1000$.

8) Options C and D are incorrect because they contradict the statements in point 7.

9) Between options A and B, B makes a stronger claim. If B is true, then A must also be true. Therefore, if we can prove B, we will have answered the question.

10) While it's difficult to calculate $f(20)$ exactly without more information, we can be certain that it is much larger than 1000 based on the rapid growth of the function.

Therefore, the correct answer is Option B: $f(20) > 1000$.
```
