## Answers to single-choice questions from Claude 3 opus
### Question 1
```
Let's approach this step-by-step:

1) Set A is defined as $A = \{x \mid -5 < x^3 < 5\}$. This means A consists of all real numbers x such that $x^3$ is between -5 and 5.

2) To find which elements of B are in A, we need to check each element of B and see if it satisfies the condition for A.

3) For -3:
   $(-3)^3 = -27$, which is not between -5 and 5. So -3 is not in A.

4) For -1:
   $(-1)^3 = -1$, which is between -5 and 5. So -1 is in A.

5) For 0:
   $0^3 = 0$, which is between -5 and 5. So 0 is in A.

6) For 2:
   $2^3 = 8$, which is not between -5 and 5. So 2 is not in A.

7) For 3:
   $3^3 = 27$, which is not between -5 and 5. So 3 is not in A.

8) Therefore, the elements of B that are also in A are -1 and 0.

9) So $A \cap B = \{-1, 0\}$

Therefore, the correct answer is Option A: ${-1, 0}$.
```
### Question 2
```
Let's solve this step-by-step.

Given: $\frac{z}{z-1} = 1 + i$

Step 1: Cross multiply.
$z = (1 + i)(z - 1)$

Step 2: Expand the right side.
$z = z - 1 + iz - i$

Step 3: Combine like terms.
$z = z + iz - 1 - i$

Step 4: Subtract $z$ from both sides.
$0 = iz - 1 - i$

Step 5: Add $1 + i$ to both sides.
$1 + i = iz$

Step 6: Divide both sides by $i$.
$\frac{1 + i}{i} = z$

Step 7: Simplify.
$-i + 1 = z$ or $1 - i = z$

Therefore, the correct answer is Option C: $1 - i$.
```
### Question 3
```
Let's approach this step-by-step:

1) For two vectors to be perpendicular, their dot product must be zero. So, we can set up an equation:

   $b \cdot (b - 4a) = 0$

2) Expanding this:

   $(2, x) \cdot (2, x - 4) = 0$

3) Calculating the dot product:

   $2 * 2 + x * (x - 4) = 0$

4) Simplifying:

   $4 + x^2 - 4x = 0$

5) Rearranging:

   $x^2 - 4x + 4 = 0$

6) This is a quadratic equation. We can solve it using the quadratic formula:

   $x = \frac{-b \pm \sqrt{b^2 - 4ac}}{2a}$

   where $a = 1$, $b = -4$, and $c = 4$

7) Substituting:

   $x = \frac{4 \pm \sqrt{(-4)^2 - 4(1)(4)}}{2(1)}$

8) Simplifying:

   $x = \frac{4 \pm \sqrt{16 - 16}}{2} = \frac{4 \pm 0}{2} = 2$

Therefore, the correct answer is Option D: $x = 2$.
```
### Question 4
```
Okay, let's approach this step-by-step using the trigonometric identities for the cosine of the sum and difference of angles, and the relation between tangent of angles.

1) We are given that $\cos(\alpha + \beta) = m$, and $\tan(\alpha) \tan(\beta) = 2$.

2) We want to find $\cos(\alpha - \beta)$.

3) We can use the identity for the cosine of the difference of angles:

   $\cos(\alpha - \beta) = \cos(\alpha) \cos(\beta) + \sin(\alpha) \sin(\beta)$

4) We don't directly know $\cos(\alpha)$, $\cos(\beta)$, $\sin(\alpha)$, or $\sin(\beta)$. But we can find them using the given information.

5) From $\tan(\alpha) \tan(\beta) = 2$, let's call $\tan(\alpha) = a$ and $\tan(\beta) = b$. Then $ab = 2$.

6) Using the identity $\tan^2(x) + 1 = \sec^2(x)$, we get:

   $a^2 + 1 = \sec^2(\alpha)$, and $b^2 + 1 = \sec^2(\beta)$

7) Therefore, $\cos(\alpha) = \frac{1}{\sqrt{a^2 + 1}}$ and $\cos(\beta) = \frac{1}{\sqrt{b^2 + 1}}$.

8) Also, $\sin(\alpha) = a \cos(\alpha) = \frac{a}{\sqrt{a^2 + 1}}$ and $\sin(\beta) = b \cos(\beta) = \frac{b}{\sqrt{b^2 + 1}}$.

9) Substituting these into the identity from step 3:

   $\cos(\alpha - \beta) = \frac{1}{\sqrt{a^2 + 1}} \cdot \frac{1}{\sqrt{b^2 + 1}} + \frac{a}{\sqrt{a^2 + 1}} \cdot \frac{b}{\sqrt{b^2 + 1}}$

   $= \frac{1 + ab}{\sqrt{(a^2 + 1)(b^2 + 1)}}$

10) We know that $ab = 2$, so:

    $\cos(\alpha - \beta) = \frac{1 + 2}{\sqrt{(a^2 + 1)(b^2 + 1)}} = \frac{3}{\sqrt{(a^2 + 1)(b^2 + 1)}}$

11) Now, we can use the identity for the cosine of the sum of angles:

    $\cos(\alpha + \beta) = \cos(\alpha) \cos(\beta) - \sin(\alpha) \sin(\beta)$

    Substituting the values from steps 7 and 8:

    $m = \frac{1}{\sqrt{a^2 + 1}} \cdot \frac{1}{\sqrt{b^2 + 1}} - \frac{a}{\sqrt{a^2 + 1}} \cdot \frac{b}{\sqrt{b^2 + 1}}$

    $= \frac{1 - ab}{\sqrt{(a^2 + 1)(b^2 + 1)}}$

    Since $ab = 2$, we get: $m = \frac{1 - 2}{\sqrt{(a^2 + 1)(b^2 + 1)}} = -\frac{1}{\sqrt{(a^2 + 1)(b^2 + 1)}}$

12) From steps 10 and 11, we can see that:

    $\cos(\alpha - \beta) = -3m$

Therefore, the correct answer is Option A: $\cos(\alpha - \beta) = -3m$.
```
### Question 5
```
Let's approach this step-by-step:

1) Let the radius of the base be $r$ for both the cylinder and the cone.

2) The lateral surface area of a cylinder is given by $2\pi rh$, where $h$ is the height. 
   Here, $h = \sqrt{3}r$. So, the lateral surface area of the cylinder is $2\pi r(\sqrt{3}r) = 2\sqrt{3}\pi r^2$.

3) The lateral surface area of a cone is given by $\pi rs$, where $s$ is the slant height. 
   We are told that the lateral surface areas of the cylinder and the cone are equal. So:

   $2\sqrt{3}\pi r^2 = \pi rs$

   $s = 2\sqrt{3}r$

4) In a cone, the slant height $s$, the radius $r$, and the height $h$ form a right-angled triangle. By Pythagoras theorem:

   $s^2 = r^2 + h^2$

   $(2\sqrt{3}r)^2 = r^2 + h^2$

   $12r^2 = r^2 + h^2$

   $11r^2 = h^2$

   $h = \sqrt{11}r$

5) The volume of a cone is given by $\frac{1}{3}\pi r^2h$. Substituting the values:

   $V = \frac{1}{3}\pi r^2(\sqrt{11}r)$

   $V = \frac{1}{3}\sqrt{11}\pi r^3$

6) We are told that the height of the cylinder is $\sqrt{3}r$. The volume of a cylinder is $\pi r^2h$. So:

   $V_{cylinder} = \pi r^2(\sqrt{3}r) = \sqrt{3}\pi r^3$

   $r^3 = \frac{V_{cylinder}}{\sqrt{3}\pi}$

7) Substituting this in the volume of the cone:

   $V = \frac{1}{3}\sqrt{11}\pi (\frac{V_{cylinder}}{\sqrt{3}\pi})$

   $V = \frac{1}{3}\sqrt{\frac{11}{3}}V_{cylinder}$

8) We are given that the volume of the cylinder is $9\sqrt{3}\pi$. So:

   $V = \frac{1}{3}\sqrt{\frac{11}{3}}(9\sqrt{3}\pi)$

   $V = 3\sqrt{11}\pi$

Therefore, the correct answer is Option B: $3\sqrt{3}\pi$.
```
### Question 6
```
Okay, let's approach this step-by-step:

1) For $f(x)$ to be strictly increasing on $R$, it needs to be strictly increasing on both $(-\infty, 0)$ and $[0, \infty)$, and it must be continuous at $x=0$.

2) For $x \geq 0$, $f(x) = e^x + \ln(x+1)$. 
   
   $\frac{d}{dx}(e^x + \ln(x+1)) = e^x + \frac{1}{x+1} > 0$ for all $x \geq 0$.

   So, $f(x)$ is always strictly increasing on $[0, \infty)$ regardless of the value of $a$.

3) For $x < 0$, $f(x) = -x^2 - 2ax - a$. 
   
   $\frac{d}{dx}(-x^2 - 2ax - a) = -2x - 2a$. 
   
   For this to be positive for all $x < 0$, we need $a < 0$.

4) Now, let's check the continuity at $x=0$. 
   
   $\lim_{x \to 0^-} (-x^2 - 2ax - a) = -a$
   
   $\lim_{x \to 0^+} (e^x + \ln(x+1)) = 1$

   For continuity, we need $-a = 1$, or $a = -1$.

5) Therefore, to ensure $f(x)$ is strictly increasing on $R$, we must have $a = -1$.

The only option that includes $a = -1$ is Option B: $[-1, 0]$.

So, the correct answer is Option B.
```
### Question 7
```
Okay, let's approach this step-by-step:

1) The intersection points occur when $\sin x = 2\sin (3x - \frac{\pi}{6})$.

2) We can solve this by equating the arguments of the sine functions (since sine is a periodic function, this will give us all the solutions).

   $x = 3x - \frac{\pi}{6}$
   $-2x = -\frac{\pi}{6}$
   $x = \frac{\pi}{12}$

   This is one solution. Let's call it $x_1$.

3) But remember, sine has a period of $2\pi$. This means that $\sin x = \sin (x + 2\pi)$. So, we can get more solutions by adding multiples of $\frac{2\pi}{3}$ to $x_1$ (because the argument of the second sine function is $3x$, so its period is $\frac{2\pi}{3}$).

   $x_2 = x_1 + \frac{2\pi}{3} = \frac{\pi}{12} + \frac{2\pi}{3} = \frac{3\pi}{4}$

   $x_3 = x_2 + \frac{2\pi}{3} = \frac{3\pi}{4} + \frac{2\pi}{3} = \frac{17\pi}{12}$

4) We don't need to go further because the next value would exceed $2\pi$.

5) So, within the range $[0, 2\pi]$, there are 3 solutions: $\frac{\pi}{12}$, $\frac{3\pi}{4}$, and $\frac{17\pi}{12}$. This means there are 3 intersection points.

Therefore, the correct answer is Option A: 3.
```
### Question 8
```
Let's think through this step-by-step:

1) We are given that $f(x) > f(x-1) + f(x-2)$ for all $x$ in the domain of $f$, which is the set of all real numbers $R$.

2) We are also given that for $x < 3$, $f(x) = x$. This gives us the base cases:
   
   $f(0) = 0$
   $f(1) = 1$
   $f(2) = 2$

3) Now, let's calculate $f(3)$. Since $3 \geq 3$, we use the relation $f(x) > f(x-1) + f(x-2)$:
   
   $f(3) > f(2) + f(1) = 2 + 1 = 3$

4) Similarly, for $f(4)$:
   
   $f(4) > f(3) + f(2) > 3 + 2 = 5$

5) We can see that the values of $f(x)$ are growing quite rapidly. In fact, they are growing faster than the Fibonacci sequence, as each term is greater than the sum of the previous two terms.

6) Without calculating the exact values, we can say that:
   
   $f(10)$ will be much larger than $55$ (the 10th Fibonacci number).
   
   $f(20)$ will be much larger than $6765$ (the 20th Fibonacci number).

7) Therefore, we can confidently say that $f(10) > 100$ and $f(20) > 1000$.

8) Options C and D are incorrect because they contradict the statements in point 7.

9) Between options A and B, B makes a stronger claim. If B is true, then A must also be true. Therefore, if we can prove B, we will have answered the question.

10) While it's difficult to calculate $f(20)$ exactly without more information, we can be certain that it is much larger than 1000 based on the rapid growth of the function.

Therefore, the correct answer is Option B: $f(20) > 1000$.
```

## Multiple choices
### Question 9
```
To solve this problem, we need to calculate the probabilities $P(X > 2)$ and $P(Y > 2)$.

For $X$, we have $\mu = 1.8$ and $\sigma = 0.1$. We can standardize the variable:
$P(X > 2) = P(\frac{X - \mu}{\sigma} > \frac{2 - 1.8}{0.1}) = P(Z > 2)$, where $Z$ is a standard normal variable.
$P(Z > 2) \approx 1 - 0.9772 = 0.0228$. This is less than both 0.2 and 0.5.

Therefore, Option A is incorrect, and Option B is correct.

For $Y$, we have $\mu = \bar{x} = 2.1$ and $\sigma = \sqrt{s^2} = \sqrt{0.01} = 0.1$. We can calculate:
$P(Y > 2) = P(\frac{Y - \mu}{\sigma} > \frac{2 - 2.1}{0.1}) = P(Z > -1)$, where $Z$ is a standard normal variable.
$P(Z > -1) \approx 1 - 0.1587 = 0.8413$. This is greater than 0.5 and 0.8.

Therefore, Option C is correct, and Option D is incorrect.

In summary, the correct options are B and C.
```

### Question 10
```
Okay, let's analyze each option one by one:

Option A: $x = 3$ is $f(x)$'s local minimum point
To check this, let's find the derivative of $f(x)$:
$f'(x) = 2(x-1)(x-4) + (x-1)^2$
$f'(x) = (x-1)(3x-6)$
At $x=3$, $f'(3) = 2 \cdot (-3) = -6 \neq 0$, so $x=3$ is not a local minimum point. 
Therefore, Option A is incorrect.

Option B: When $0 < x < 1$, $f(x) < f(x^2)$
Let $0 < x < 1$. Then $x^2 < x$.
Since $0 < x < 1$, $-1 < x-1 < 0$ and $-4 < x-4 < -3$. 
So, $(x-1)^2 > 0$ and $(x-4) < 0$. Therefore, $f(x) < 0$.
Since $0 < x^2 < x < 1$, by the same reasoning, $f(x^2) < 0$ as well.
But since $x^2 < x$, $|x-1| > |x^2-1|$ and $|x-4| > |x^2-4|$, so $f(x) < f(x^2)$.
Therefore, Option B is correct.

Option C: When $1 < x < 2$, $-4 < f(2x - 1) < 0$
Let $1 < x < 2$. Then $1 < 2x-1 < 3$ and $-2 < 2x-5 < -1$.
So, $0 < (2x-2)^2$ and $-2 < 2x-5 < -1$, meaning $f(2x-1) < 0$.
Also, $f(2x-1) = (2x-2)^2(2x-5) > -4$ because $(2x-2)^2 < 4$ and $2x-5 > -2$.
Therefore, Option C is correct.

Option D: When $-1 < x < 0$, $f(2 - x) > f(x)$
Let $-1 < x < 0$. Then $2 < 2-x < 3$ and $-2 < x-1 < -1$.
So, $f(x) = (x-1)^2(x-4) > 0$ because $(x-1)^2 > 0$ and $(x-4) < 0$.
Also, $f(2-x) = (1-x)^2(-2-x) < 0$ because $(1-x)^2 > 0$ and $(-2-x) < 0$.
Therefore, $f(2-x) < 0 < f(x)$, so $f(2 - x) < f(x)$.
Therefore, Option D is incorrect.

In conclusion, only Option B and Option C are correct.
```

### Question 11
```
Let's solve this step by step:

1) The given information suggests that the curve $C$ is a hyperbola with foci at $O(0,0)$ and $F(2,0)$, and a vertical transverse axis.

2) The equation of such a hyperbola is of the form $\frac{x^2}{a^2} - \frac{y^2}{b^2} = 1$, where $a$ and $b$ are the distances from the center to the vertices and co-vertices respectively.

3) Given that the product of the distances from $O$ to $F$ and from $O$ to the line $x = a$ is 4, we can write:

   $2 \cdot (-a) = 4$
   $a = -2$

   So, Option A is correct.

4) If $a = -2$, then the vertices of the hyperbola are at $(-2,0)$ and $(2,0)$. The point $(2\sqrt{2}, 0)$ is outside the interval $[-2,2]$, so it does not lie on the hyperbola.

   Therefore, Option B is incorrect.

5) The vertical asymptotes of the hyperbola are at $x = \pm a = \pm 2$. There is no vertical asymptote at $x = 1$.

   Thus, Option C is incorrect.

6) For any point $(x_0, y_0)$ on the hyperbola, we have:

   $\frac{x_0^2}{a^2} - \frac{y_0^2}{b^2} = 1$

   Substituting $a = 2$ and rearranging:

   $y_0^2 = b^2(\frac{x_0^2}{4} - 1) = (\frac{b^2}{4})(x_0 - 2)(x_0 + 2)$

   Taking the square root and considering the positive branch (as $y_0 \leq \frac{4}{x_0 + 2}$ is given):

   $y_0 = \frac{b}{2}\sqrt{(x_0 - 2)(x_0 + 2)}$

   For this to be less than or equal to $\frac{4}{x_0 + 2}$ for all $x_0$, we must have $b \leq 4$.

   Therefore, Option D is correct if $b \leq 4$, but we don't have enough information to determine this.

In conclusion, Option A is definitely correct, Option D may be correct depending on the value of $b$, while Options B and C are incorrect.
```

## Fill-in-the-blank 
### Question 12
```
Okay, let's approach this step-by-step:

1) In a hyperbola, the difference of the distances from any point on the hyperbola to the two foci is constant and equal to the transverse axis (which is $2a$ in this case).

2) Let's say the point $A$ is closer to $F_1$ than $F_2$. Then,

   $|F_2A| - |F_1A| = 2a$

3) We are given that $|F_1A| = 13$ and $|AB| = 10$. Since $F_2$ is on the line $AB$, we can say:

   $|F_2A| = |F_1A| + |AB| = 13 + 10 = 23$

4) Substituting in the equation from step 2:

   $23 - 13 = 2a$
   $10 = 2a$
   $a = 5$

5) The eccentricity of a hyperbola is defined as:

   $e = \sqrt{1 + \frac{b^2}{a^2}}$

6) To find $b$, we can use the fact that the distance from the center to either focus is $\sqrt{a^2 + b^2}$. Since the line $AB$ passes through the right focus and is parallel to the y-axis, the x-coordinate of the right focus is $a$. Therefore, the distance from the center to the right focus is just $a$.

   $a = \sqrt{a^2 + b^2}$
   $5 = \sqrt{25 + b^2}$
   $25 = 25 + b^2$
   $b^2 = 0$
   $b = 0$

7) Now we can calculate the eccentricity:

   $e = \sqrt{1 + \frac{0^2}{5^2}} = \sqrt{1 + 0} = 1$

Therefore, the eccentricity of the hyperbola is 1.
```

### Question 13
```
Let's solve this step by step:

1) First, let's find the equation of the tangent line to the curve $y = e^x + x$ at the point $(0, 1)$. To do this, we need to find the derivative of this function at $x = 0$.

   $\frac{d}{dx}(e^x + x) = e^x + 1$
   At $x = 0$, $e^0 + 1 = 2$

   So the slope of the tangent line at $(0, 1)$ is 2.

2) The equation of a line with slope $m$ passing through a point $(x_1, y_1)$ is $y - y_1 = m(x - x_1)$. Here, $m = 2$, $x_1 = 0$, and $y_1 = 1$. So the equation of the tangent line is:

   $y - 1 = 2(x - 0)$
   $y = 2x + 1$

3) Now, let's consider the curve $y = \ln(x+1) + a$. The tangent line to this curve will have the same slope as the curve at the point of tangency. Let's call this point of tangency $(x_0, y_0)$. The slope of this curve at any point is given by its derivative:

   $\frac{d}{dx}(\ln(x+1) + a) = \frac{1}{x+1}$

   For the tangent line to be the same as the one we found earlier, this slope must equal 2 at the point of tangency. So:

   $\frac{1}{x_0+1} = 2$
   $x_0 + 1 = \frac{1}{2}$
   $x_0 = -\frac{1}{2}$

4) Now that we know $x_0$, we can find $y_0$ by plugging $x_0$ into the equation of the second curve:

   $y_0 = \ln(-\frac{1}{2}+1) + a = \ln(\frac{1}{2}) + a$

5) Since $(x_0, y_0)$ is on the tangent line, it must satisfy the equation of the tangent line:

   $y_0 = 2x_0 + 1$
   $\ln(\frac{1}{2}) + a = 2(-\frac{1}{2}) + 1$
   $\ln(\frac{1}{2}) + a = 0$
   $a = -\ln(\frac{1}{2}) = \ln(2)$

Therefore, the value of the constant $a$ is $\ln(2)$.
```

### Question 14
```
Let's approach this step-by-step:

1) First, let's find the total number of possible outcomes. In each round, A has 4 choices, and B has 4 choices, so there are 4 * 4 = 16 possible outcomes per round. Since there are 4 rounds, and the choices in each round are independent, there are 16^4 = 65,536 total possible outcomes.

2) Now, let's consider the ways in which A can score at least 2 points. A can score 2, 3, or 4 points.

3) If A scores 4 points, they must win all 4 rounds. There is only 1 way for this to happen: A must choose 7, 5, 3, 1 in that order, while B chooses 8, 6, 4, 2 in that order. So there is 1 way for A to score 4 points.

4) If A scores 3 points, they must win 3 rounds and lose 1 round. There are 4 choose 1 = 4 ways to choose the round that A loses, and for each of these, there is only 1 way for the cards to be chosen (similar to step 3). So there are 4 ways for A to score 3 points.

5) If A scores 2 points, they must win 2 rounds and lose 2 rounds. There are 4 choose 2 = 6 ways to choose the rounds that A wins. For each of these 6 ways, there are 2 ways for the cards to be chosen in each round (A can choose the higher of their remaining two cards, or the lower). So there are 6 * 2^4 = 96 ways for A to score 2 points.

6) Adding these up, there are 1 + 4 + 96 = 101 ways for A to score at least 2 points.

7) Therefore, the probability that A's total score is at least 2 is 101 / 65,536 = 0.001541... or about 0.15%.
```
