## Answers to single-choice questions from Gemini_ultra_1.0
### Question 1
```
The correct answer is **Option A: {-1, 0}**. Here's why:

* **Set A:**  The inequality $-5 < x^3 < 5$ means we need to find the values of x whose cubes are between -5 and 5. The only integers that satisfy this are -1, 0, and 1.  So, set A = {-1, 0, 1}.
* **Set B:**  This set is given as {-3, -1, 0, 2, 3}.
* **Intersection (A ∩ B):** The intersection of two sets includes only the elements that are in both sets.  Therefore, A ∩ B = {-1, 0}.
```
### Question 2
```
We can solve for $z$ directly:

$$\frac{z}{z-1} = 1+i$$

$$z = (1+i)(z-1)$$

$$z = z - 1 + iz - i$$

$$1 - i = iz$$

$$z = \frac{1-i}{i}$$

Multiplying the numerator and denominator by $-i$ (the conjugate of $i$):

$$z = \frac{(1-i)(-i)}{i(-i)}$$

$$z = \frac{-i -1}{1}$$

$$z = -1 - i$$

**Therefore, the correct answer is Option A.**
```
### Question 3
```
Here's how to solve the problem:

**Understanding Perpendicular Vectors**

Two vectors are perpendicular if their dot product is zero.  

**Calculations**

1. **Find b - 4a:** 
   (b - 4a) = (2, x) - 4(0, 1) = (2, x - 4)

2. **Calculate the dot product of b and (b - 4a):**
   b ⋅ (b - 4a) = (2, x) ⋅ (2, x - 4) = 4 + x(x - 4)

3. **Set the dot product to zero (since b and b - 4a are perpendicular):**
   4 + x(x - 4) = 0

4. **Solve the quadratic equation:**
   x² - 4x + 4 = 0
   (x - 2)² = 0
   x = 2

**Answer**

The correct answer is **Option D: 2**
```
### Question 4
```
Here's how to solve the problem and find the correct option:

**Key Trigonometric Identities**

We'll use the following trigonometric identities:

* **Cosine of Sum/Difference:**
   *  cos(α + β) = cosα cosβ - sinα sinβ
   *  cos(α - β) = cosα cosβ + sinα sinβ

* **Tangent:**
   *  tanα = sinα / cosα

**Solution**

1. **Express tanα tanβ in terms of cosines:**

   Since tanα tanβ = 2, we have (sinα / cosα)(sinβ / cosβ) = 2.
   This simplifies to sinα sinβ = 2 cosα cosβ.

2. **Manipulate the cos(α + β) equation:**

   We know cos(α + β) = m = cosα cosβ - sinα sinβ.
   Substitute the result from step 1:  m = cosα cosβ - 2 cosα cosβ.
   This simplifies to -m = cosα cosβ.

3. **Find cos(α - β):**

   cos(α - β) = cosα cosβ + sinα sinβ
   Substitute the values we found: cos(α - β) = -m + 2(-m) = -3m

**Answer**

The correct option is **Option A: -3m**.
```
### Question 5
```
Here's how to solve the problem and determine the correct answer:

**1. Formulas:**

* **Lateral Surface Area of a Cylinder:**  2πrh (r = radius, h = height)
* **Lateral Surface Area of a Cone:** πrl (r = radius, l = slant height)
* **Volume of a Cone:** (1/3)πr²h (r = radius, h = height)

**2. Given Information:**

* Radius of cylinder (r) = √3
* Height of cylinder (h) = √3
* Lateral surface areas of the cylinder and cone are equal.

**3. Finding the Slant Height of the Cone (l):**

* Set the lateral surface areas equal: 2πrh = πrl
* Cancel π and r on both sides: 2h = l
* Substitute h = √3: 2√3 = l

**4. Finding the Height of the Cone:**

* Use the Pythagorean theorem: l² = r² + h²
* Substitute l = 2√3 and r = √3: (2√3)² = (√3)² + h²
* Simplify and solve for h: 12 = 3 + h²  =>  h² = 9  =>  h = 3

**5. Calculating the Volume of the Cone:**

* Volume = (1/3)πr²h
* Substitute r = √3 and h = 3: (1/3)π(√3)²(3)
* Simplify: (1/3)π(3)(3) = 3π

**Answer:**

The correct answer is **Option B: 3√3π**
```
### Question 6
```
Here's how to determine the correct answer:

**Understanding the Problem**

A strictly increasing function means its derivative is always positive. We need to find the range of 'a' that ensures this condition for both parts of the piecewise function.

**Analyzing the Function**

* **For x < 0:**
   The derivative is  f'(x) = -2x - 2a. For this to be positive when x is negative, we need -2a > 0, which implies a < 0.

* **For x ≥ 0:**
    The derivative is f'(x) = e^x + 1/(x+1). This is always positive since both e^x and 1/(x+1) are positive for x ≥ 0.

**Critical Point at x = 0**

We need to ensure the function is continuous and differentiable at x = 0.  

* **Continuity:** The left and right limits at x = 0 must be equal:
    * lim (x->0-) f(x) = -a
    * lim (x->0+) f(x) = 1
    * This implies -a = 1, so a = -1

* **Differentiability:** The left and right derivatives at x = 0 must be equal:
    * lim (x->0-) f'(x) = -2a
    * lim (x->0+) f'(x) = 2
    * This implies -2a = 2, so a = -1

**Combining the Conditions**

* We need a < 0 to ensure the first part of the function is strictly increasing.
* We need a = -1 to ensure continuity and differentiability at x = 0.

**The Answer**

The only value of 'a' that satisfies all conditions is a = -1. Since this is the only possible value, the range of 'a' is a single point. 

**Therefore, the correct answer is none of the given options.**
```
### Question 7
```
**Option C: 6** is the correct answer.

**Explanation:**

While graphing these functions is a helpful visualization, we can solve this problem analytically. We want to find the values of *x* for which:

```
sin x = 2 sin(3x - π/6)
```

Using the angle subtraction formula for sine, we get:

```
sin x = 2 (sin 3x cos π/6 - cos 3x sin π/6)
sin x = √3 sin 3x - cos 3x 
```

Using the triple angle formula for sine and cosine, we get:

```
sin x = √3 (3 sin x - 4 sin^3 x) - (4 cos^3 x - 3 cos x)
```

Let's substitute *s = sin x* and *c = cos x*.  Remember that *s² + c² = 1*. After some simplification, we get:

```
4s^3 - 3s + 4c^3 - 3c = 0
(s + c)(4s^2 - 4sc + 4c^2 - 3) = 0
```

This gives us two possibilities:

1. **s + c = 0**:  This means sin x + cos x = 0.  There are two solutions to this in the interval [0, 2π].

2. **4s² - 4sc + 4c² - 3 = 0**:  Dividing by 4 and using the identity s² + c² = 1, we get: 1 - sc = 3/4.  Then, sc = 1/4. Squaring both sides and using the identity again, we get a quadratic in s² which has four solutions in the interval [0, 2π].

Therefore, there are a total of **6** intersection points.
```
### Question 8
```
Here's how we can solve this problem:

**Understanding the Problem**

* We have a function defined for all real numbers.
* The function has a special property: its value at any point is greater than the sum of its values at the two previous integers.
* For values less than 3, the function is simply the identity function (f(x) = x).

**Strategy**

We'll use the given information to calculate some initial values of the function and see if we can spot a pattern that helps us determine which option is correct.

**Calculations**

* **f(0) = 0**  (Since 0 < 3)
* **f(1) = 1**  (Since 1 < 3)
* **f(2) = 2**  (Since 2 < 3)
* **f(3) > f(2) + f(1) = 3**
* **f(4) > f(3) + f(2) > 5**
* **f(5) > f(4) + f(3) > 8**

Notice that the function values are growing quickly. Let's continue:

* **f(6) > f(5) + f(4) > 13**
* **f(7) > f(6) + f(5) > 21**
* **f(8) > f(7) + f(6) > 34**

**The Pattern**

We can see that the function values are growing faster than the Fibonacci sequence (0, 1, 1, 2, 3, 5, 8, 13...).  Since the Fibonacci sequence grows exponentially, it's reasonable to expect that f(x) will also grow very quickly.

**Eliminating Options**

* **Option A:**  f(10) > 100 is likely true, but we need to check the other options.
* **Option C:** f(10) < 1000 seems very unlikely given the rapid growth we've observed.
* **Option D:** f(20) < 10000 also seems unlikely due to the exponential growth.

**Focusing on Option B**

Let's see if f(20) could be greater than 1000.  We know f(8) > 34. If we continue the pattern, we would expect:

* f(9) > 55
* f(10) > 89
* ...
* f(20) would be much greater than 1000.

**Answer**

The most likely correct answer is **Option B: f(20) > 1000**. 

```
## Multiple choices
### Question 9
```
Here's how we analyze each option:

**Option A: P(X > 2) > 0.2**

* Standardize X:  Z = (X - 1.8) / 0.1
* P(X > 2) = P(Z > (2 - 1.8)/0.1) = P(Z > 2)
* Since P(Z < 2) ≈ 0.9772, P(Z > 2) ≈ 1 - 0.9772 = 0.0228
* 0.0228 is not greater than 0.2, so Option A is incorrect.

**Option B: P(X > 2) < 0.5**

* From the calculation above, P(X > 2) ≈ 0.0228
* 0.0228 is less than 0.5, so Option B is correct.

**Option C: P(Y > 2) > 0.5**

* Standardize Y: Z = (Y - 2.1) / 0.1 (since the standard deviation of Y is the square root of the variance)
* P(Y > 2) = P(Z > (2 - 2.1)/0.1) = P(Z > -1)
* Since P(Z < -1) ≈ 0.1587, P(Z > -1) ≈ 1 - 0.1587 = 0.8413
* 0.8413 is greater than 0.5, so Option C is correct.

**Option D: P(Y > 2) < 0.8**

* From the calculation above, P(Y > 2) ≈ 0.8413
* 0.8413 is not less than 0.8, so Option D is incorrect.

**Conclusion**

The correct options are **B** and **C**.
```

### Question 10
```
Here's the analysis for each option:

**Option A: $x = 3$ is $f(x)$'s local minimum point**

* **Correct.** To determine local extrema, we can find the critical points by taking the derivative and setting it equal to zero:
   
   ```
   f'(x) = 2(x - 1)(x - 4) + (x - 1)^2 = (x - 1)(3x - 7)
   ```

   Setting f'(x) = 0, we get x = 1 and x = 7/3. We can use the second derivative test to confirm that x = 7/3 (or approximately x = 2.33) is a local minimum. Since 3 is close to 2.33, it is also the x-coordinate of the local minimum point.

**Option B: When $0 < x < 1$, $f(x) < f(x^2)$**

* **Incorrect.** In the interval (0, 1), x^2 is smaller than x.  Since f(x) is decreasing before x = 1, f(x) will be greater than f(x^2) for values of x in this interval.

**Option C: When $1 < x < 2$, $-4 < f(2x - 1) < 0$**

* **Correct.** If 1 < x < 2, then 1 < 2x - 1 < 3.  In this interval, f(x) is negative.  Since f(x) is a continuous function, f(2x - 1) will take on all values between f(1) = 0 and f(3) = -4.

**Option D: When $-1 < x < 0$, $f(2 - x) > f(x)$**

* **Correct.** If -1 < x < 0, then 2 < 2 - x < 3. Since the graph of f(x) is symmetric about the vertical line x = 1, f(2 - x) will have the same value as f(x - 2). In the interval -1 < x < 0, f(x - 2) will be negative while f(x) will be positive.

**Therefore, the correct options are A, C, and D.**
```

### Question 11
```
Here's the breakdown of why the correct options are A and D:

**Understanding the Problem**

The problem describes a curve *C* with these properties:

1. **Passes through origin:**  The curve goes through the point (0, 0).
2. **x-coordinate restriction:** All x-values on the curve are greater than -2.
3. **Distance product:**  The product of the distance from the origin to the point (2, 0) and the distance from the origin to the line x = *a* is 4.

**Analyzing the Options**

* **Option A: a = -2**
   * The distance from the origin to (2, 0) is 2.
   * The distance from the origin to the line x = -2 is 2.
   * Their product is 4.  
   * **This option is correct.**

* **Option B: The point (2√2, 0) lies on C**
   * There's no information given in the problem to suggest this point would be on the curve.
   * **This option is incorrect.**

* **Option C: C in the first quadrant has a vertical asymptote at x = 1**
   *  The problem doesn't provide any information about asymptotes.
   * **This option is incorrect.**

* **Option D: when the point (x₀, y₀) lies on C, then y₀ ≤ 4/(x₀ + 2)**
   * Consider the distance product condition. Let the distance from the origin to (x₀, y₀) be *d*. Then:
      * *d* * |-a| = 4 
      * *d* = 4/|-a|
   * Since *a* is negative, |-a| = -a
   * *d* = 4/(-a)
   * By the distance formula, *d* = √(x₀² + y₀²)
   * So, √(x₀² + y₀²) = 4/(-a)
   * Squaring both sides: x₀² + y₀² = 16/a²
   * Rearranging: y₀² = 16/a² - x₀²
   * Since the curve is to the right of x = -2, we know x₀ > -2. Therefore:
      * x₀ + 2 > 0
      * Squaring both sides: (x₀ + 2)² > 0
      * Expanding: x₀² + 4x₀ + 4 > 0
      * Rearranging: -x₀² - 4x₀ - 4 < 0
      * Adding 16/a² to both sides: 16/a² - x₀² - 4x₀ - 4 < 16/a²
      * Factoring: (4/(x₀ + 2))² < 16/a²
      * Since everything is positive, we can take the square root: 4/(x₀ + 2) < 4/(-a)
      * Multiplying both sides by -a(x₀ + 2): y₀ < 4/(x₀ + 2)
   * **This option is correct.**

**Answer**
The correct options are A and D.
```

## Fill-in-the-blank 
### Question 12
```
Here's a step-by-step solution:

**1. Understand the Hyperbola Properties**

* **Foci:** For a hyperbola, the foci are points $F_1(-c,0)$ and $F_2(c,0)$, where $c^2 = a^2 + b^2$.
* **Definition:** The difference between the distances from any point on the hyperbola to the two foci is constant and equal to $2a$.

**2. Visualize the Problem**

[Image of a hyperbola with center at the origin, opening left and right, with foci labeled F1 and F2. A vertical line passes through F2, intersecting the hyperbola at points A and B.]

**3. Set up Equations**

* Let $A$ be the point $(c, y)$ on the hyperbola (since it lies on the vertical line through $F_2$).
* Using the definition of a hyperbola:  
   * $|AF_1| - |AF_2| = 2a$
* We are given $|AF_1| = 13$ and $|AB| = 10$. Since $F_2$ lies between $A$ and $B$, we have $|AF_2| = |AB|/2 = 5$.

**4. Solve for 'a'**

Substitute the given values into the equation:

```
13 - 5 = 2a
8 = 2a
a = 4
```

**5. Find the Coordinates of A**

Since $A$ lies on the hyperbola, we can substitute its coordinates into the hyperbola equation:

```
(c^2)/(a^2) - (y^2)/(b^2) = 1
(c^2)/(4^2) - (y^2)/(b^2) = 1 
```

Also, since $A$ is on the vertical line through $F_2$, its x-coordinate is $c$.

**6. Use the Distance Formula**

We know $|AF_1| = 13$. Using the distance formula between $A(c,y)$ and $F_1(-c,0)$:

```
sqrt((c - (-c))^2 + (y - 0)^2) = 13
sqrt((2c)^2 + y^2) = 13
```

**7. Solve for 'c' and 'b'**

Now we have two equations:

```
(c^2)/16 - (y^2)/(b^2) = 1    
4c^2 + y^2 = 169
```

Solve this system of equations (e.g., by elimination) to find:

```
c = 5
y^2 = 69
b^2 = 69/3 = 23
```

**8. Calculate the Eccentricity**

The eccentricity of a hyperbola is given by:

```
e = c/a = 5/4
```

**Therefore, the eccentricity of the hyperbola C is 5/4.**
```

### Question 13
```
Here's how to solve the problem:

**1. Find the slope of the tangent line to the first curve:**

* Differentiate the first curve:  
   
   ```
   y = e^x + x 
   dy/dx = e^x + 1
   ```

* Evaluate the derivative at x = 0 (the x-coordinate of the point of tangency):
   
   ```
   dy/dx (at x=0) = e^0 + 1 = 2
   ```
   
   This means the slope of the tangent line to the first curve at (0,1) is 2.

**2. Find the x-coordinate of the point of tangency on the second curve:**

* Differentiate the second curve:

   ```
   y = ln(x + 1) + a
   dy/dx = 1/(x + 1)
   ```

* Since the tangent lines to both curves are the same, their slopes are equal. Set the derivative of the second curve equal to 2 and solve for x:

   ```
   1/(x + 1) = 2
   x + 1 = 1/2
   x = -1/2
   ```

**3. Find the y-coordinate of the point of tangency on the second curve:**

* Substitute x = -1/2 into the equation of the second curve:

   ```
   y = ln(-1/2 + 1) + a
   y = ln(1/2) + a
   ```

**4. Use the point-slope form to find the equation of the tangent line:**

* We know the slope of the tangent line is 2, and it passes through (0,1). Using the point-slope form, the equation of the tangent line is:

   ```
   y - 1 = 2(x - 0)
   y = 2x + 1
   ```

**5. Find the value of a:**

* Since the tangent line also passes through the point (-1/2, ln(1/2) + a) on the second curve, substitute these coordinates into the equation of the tangent line:

   ```
   ln(1/2) + a = 2(-1/2) + 1
   ln(1/2) + a = 0
   a = -ln(1/2) = ln(2)
   ```

**Therefore, the value of the constant a is ln(2).**
```

### Question 14
```
Here's a solution to the problem:

**Reasoning:**

Since each player only has four cards, the four rounds essentially represent a 1-to-1 matching of A's cards with B's cards.  For A to get at least 2 points, they need to win at least two of these match-ups.

**Possible Winning Scenarios for A:**

* **Scenario 1:** A wins all four rounds.
* **Scenario 2:** A wins three rounds and loses one.
* **Scenario 3:** A wins two rounds and loses two.

Let's calculate the probability of each scenario:

* **Scenario 1:** The probability of A winning the first round is 4/4 (since any of A's cards beat any of B's cards).  The probability of winning the second round is then 3/3, and so on. So, the probability of Scenario 1 is (4/4)*(3/3)*(2/2)*(1/1) = 1.

* **Scenario 2:**  To calculate the probability of this scenario, we need to consider the different ways A can win three rounds. They could win the first three, the last three, or any other combination.  Let's consider one specific case where A wins the first three rounds. The probability of this is (4/4)*(3/3)*(2/2)*(0/1) = 0 (since A must lose the last round).  There are 4 ways to choose which round A loses, so the probability of Scenario 2 is 4 * 0 = 0.

* **Scenario 3:** There are  ⁶C₂ = 15 ways to choose which two rounds A wins.  For any specific choice of two winning rounds, the probability is the same as the probability of winning the first two rounds and losing the last two, which is (4/4)*(3/3)*(0/2)*(0/1) = 0.  Therefore, the probability of Scenario 3 is 15 * 0 = 0.

**Total Probability:**

The total probability of A getting at least 2 points is the sum of the probabilities of the three scenarios: 1 + 0 + 0 = 1.

**Conclusion:**

The probability that A's total score is at least 2 after four rounds is **1**. This means A is guaranteed to win at least two rounds. 

```
