## Answers to single-choice questions from Llama 3 70b 
### Question 1
```

To find $A \cap B$, we need to find the elements of $B$ that satisfy the condition $-5 < x^3 < 5$.
Let's check each element of $B$:
* $-3$: $(-3)^3 = -27 < -5$, so it doesn't satisfy the condition.
* $-1$: $(-1)^3 = -1$, which satisfies the condition.
* $0$: $0^3 = 0$, which satisfies the condition.
* $2$: $2^3 = 8 > 5$, so it doesn't satisfy the condition.
* $3$: $3^3 = 27 > 5$, so it doesn't satisfy the condition.
Therefore, the elements of $B$ that satisfy the condition are $-1$ and $0$. So, the correct answer is:
Option A: ${-1, 0}$

```
### Question 2
```
Let's solve for z:
\begin{align*}
\frac{z}{z-1} &= 1 + i \\
z &= (1 + i)(z - 1) \\
z &= z - 1 + iz - i \\
z - iz &= -1 + i \\
z(1 - i) &= -1 + i \\
z &= \frac{-1 + i}{1 - i} \\
z &= \frac{-1 + i}{1 - i} \cdot \frac{1 + i}{1 + i} \\
z &= \frac{-1 + i + i - i^2}{1 - i^2} \\
z &= \frac{-1 + 2i + 1}{2} \\
z &= \frac{2i}{2} \\
z &= i
\end{align*}
However, none of the options match our result. The correct answer is $i$, but it's not among the options.

```
### Question 3
```
Let's break it down step by step.
We are given two vectors: `a = (0, 1)` and `b = (2, x)`. We need to find the value of `x` such that `b` is perpendicular to `(b - 4a)`.
First, let's calculate `b - 4a`:
```
b - 4a = (2, x) - 4(0, 1) = (2, x) - (0, 4) = (2, x - 4)
```
Now, we are told that `b` is perpendicular to `(b - 4a)`, which means their dot product is zero:
```
b · (b - 4a) = 0
```
Expanding the dot product, we get:
```
(2, x) · (2, x - 4) = 0
2(2) + x(x - 4) = 0
4 + x^2 - 4x = 0
x^2 - 4x + 4 = 0
(x - 2)^2 = 0
x - 2 = 0
x = 2
```
So, the correct answer is:
Option D: `2`
```
### Question 4
```
To solve this problem, we can use the trigonometric identity for $\cos(\alpha - \beta)$:

$$\cos(\alpha - \beta) = \cos(\alpha)\cos(\beta) + \sin(\alpha)\sin(\beta)$$

We are given that $\cos(\alpha + \beta) = m$, so we can use another trigonometric identity to express $\cos(\alpha + \beta)$ in terms of $\cos(\alpha)$, $\cos(\beta)$, $\sin(\alpha)$, and $\sin(\beta)$:

$$\cos(\alpha + \beta) = \cos(\alpha)\cos(\beta) - \sin(\alpha)\sin(\beta) = m$$

Now, we can add the two equations to eliminate the $\sin(\alpha)\sin(\beta)$ term:

$$2\cos(\alpha)\cos(\beta) = m + \cos(\alpha - \beta)$$

We are also given that $\tan(\alpha)\tan(\beta) = 2$. Using the fact that $\tan(\theta) = \frac{\sin(\theta)}{\cos(\theta)}$, we can rewrite this equation as:

$$\frac{\sin(\alpha)\sin(\beta)}{\cos(\alpha)\cos(\beta)} = 2$$

Cross-multiplying, we get:

$$\sin(\alpha)\sin(\beta) = 2\cos(\alpha)\cos(\beta)$$

Substituting this into our previous equation, we get:

$$2\cos(\alpha)\cos(\beta) = m + \cos(\alpha - \beta)$$
$$\sin(\alpha)\sin(\beta) = m + \cos(\alpha - \beta)$$

Subtracting the two equations, we get:

$$\sin(\alpha)\sin(\beta) - 2\cos(\alpha)\cos(\beta) = 0$$
$$\cos(\alpha - \beta) - m = 0$$
$$\cos(\alpha - \beta) = m$$

However, this is not among the options. But we can see that none of the options are correct, as $\cos(\alpha - \beta)$ is equal to $m$, not $-3m$, $-\frac{m}{3}$, $\frac{m}{3}$, or $3m$.

So, the correct answer is "None of the above".
```
### Question 5
```
Let's break down the problem step by step:
1. The radius of the base of the cylinder and the cone are equal, so let's call this radius "r".
2. The lateral surface areas of the cylinder and the cone are equal. The lateral surface area of a cylinder is 2πrh, where h is the height of the cylinder. The lateral surface area of a cone is πrl, where l is the slant height of the cone. Since they are equal, we can set up the equation:
2πrh = πrl
We are given that the height of the cylinder is √3, so h = √3. We can simplify the equation:
2πr√3 = πrl
Now, divide both sides by πr:
2√3 = l
So, the slant height of the cone is 2√3.
3. The volume of a cone is given by the formula:
V = (1/3)πr²h
We know the radius r, and we need to find the height h of the cone. We can use the Pythagorean theorem to find the height of the cone:
h² + r² = l²
Substitute the values we know:
h² + r² = (2√3)²
h² + r² = 12
Since the height of the cylinder is √3, we can assume that the radius is also √3 (since the radius of the base of the cylinder and the cone are equal). So, r = √3. Substitute this value:
h² + (√3)² = 12
h² + 3 = 12
Subtract 3 from both sides:
h² = 9
Take the square root of both sides:
h = √9 = 3
Now that we have the height of the cone, we can find the volume:
V = (1/3)π(√3)²(3)
V = (1/3)π(3)(3)
V = 3√3π
So, the correct answer is Option B: 3√3π.
```
### Question 6
```
To ensure that f(x) is strictly increasing on R, the derivative f'(x) must be greater than 0. We can calculate the derivative as follows:
For x < 0:
f'(x) = -2x - 2a > 0
For x ≥ 0:
f'(x) = e^x + 1/(x+1) > 0 (this is always true)
Now, we need to find the range of a such that -2x - 2a > 0 for all x < 0.
Since x < 0, -2x > 0. Therefore, we need -2a > 0, which implies a < 0.
So, the correct answer is Option A: (-∞, 0].
```
### Question 7
```
The correct answer is Option C: $6$.
Explanation:
To find the number of intersection points between the curves y = sin(x) and y = 2sin(3x - π/6), we need to find the values of x that satisfy both equations.
We can start by rewriting the second equation as:
y = 2sin(3x - π/6) = 2sin(3(x - π/18))
Now, we can equate the two equations:
sin(x) = 2sin(3(x - π/18))
This equation has multiple solutions, and we can find them by using the following identity:
sin(a) = sin(b) => a = b + 2kπ or a = π - b + 2kπ, where k is an integer.
Applying this identity to our equation, we get:
x = 3(x - π/18) + 2kπ or x = π - 3(x - π/18) + 2kπ
Simplifying these equations, we get:
x = π/2 + 2kπ/5 or x = 5π/6 + 2kπ/5
Now, we need to find the values of x that lie within the interval [0, 2π]. We can do this by iterating over the values of k:
For k = 0, we get x = π/2 and x = 5π/6, which are both within the interval.
For k = 1, we get x = 9π/10 and x = 13π/10, which are both within the interval.
For k = 2, we get x = 17π/10 and x = 21π/10, which are both within the interval.
For k = 3, we get x = 25π/10 and x = 29π/10, which are both outside the interval.
Therefore, we have a total of 6 intersection points: x = π/2, x = 5π/6, x = 9π/10, x = 13π/10, x = 17π/10, and x = 21π/10.
Hence, the correct answer is Option C: 6.
```
### Question 8
```
Let's analyze the given information:
1. $f(x) > f(x-1) + f(x-2)$ for all $x$.
2. $f(x) = x$ for $x < 3$.
We can start by finding $f(3)$:
$f(3) > f(2) + f(1) = 2 + 1 = 3$, so $f(3) > 3$.
Now, let's find $f(4)$:
$f(4) > f(3) + f(2) > 3 + 2 = 5$, so $f(4) > 5$.
Similarly, we can find $f(5)$:
$f(5) > f(4) + f(3) > 5 + 3 = 8$, so $f(5) > 8$.
We can continue this process to find:
$f(6) > 13$, $f(7) > 21$, $f(8) > 34$, $f(9) > 55$, and $f(10) > 89$.
Now, let's look at the options:
Option A: $f(10) > 100$ is false, since we found $f(10) > 89$.
Option B: $f(20) > 1000$ is true, since $f(20)$ will be much larger than 1000 due to the recursive nature of the function.
Option C: $f(10) < 1000$ is true, since we found $f(10) > 89$.
Option D: $f(20) < 10000$ is false, since $f(20)$ will be much larger than 10000.
The correct answer is Option B: $f(20) > 1000$.
```
## Multiple choices
### Question 9
```
Let's break down the problem step by step:

1. We know that $X$ follows a normal distribution $N(1.8, 0.1^2)$. To find $P(X > 2)$, we can standardize the value 2 using the z-score formula:

$$z = \frac{2 - 1.8}{0.1} = 2$$

Using a standard normal distribution table or calculator, we find that $P(Z > 2) \approx 0.0228$. Since $X$ has a normal distribution, we can conclude that $P(X > 2) \approx 0.0228$.

Comparing this result to the options:

* Option A: $P(X > 2) > 0.2$ is incorrect since $P(X > 2) \approx 0.0228 < 0.2$.
* Option B: $P(X > 2) < 0.5$ is correct since $P(X > 2) \approx 0.0228 < 0.5$.

2. We know that $Y$ follows a normal distribution $N(2.1, 0.01)$. To find $P(Y > 2)$, we can standardize the value 2 using the z-score formula:

$$z = \frac{2 - 2.1}{\sqrt{0.01}} = -1$$

Using a standard normal distribution table or calculator, we find that $P(Z > -1) \approx 0.8413$. Since $Y$ has a normal distribution, we can conclude that $P(Y > 2) \approx 0.8413$.

Comparing this result to the options:

* Option C: $P(Y > 2) > 0.5$ is correct since $P(Y > 2) \approx 0.8413 > 0.5$.
* Option D: $P(Y > 2) < 0.8$ is correct since $P(Y > 2) \approx 0.8413 < 0.8$.

Therefore, the correct options are:

* Option B: $P(X > 2) < 0.5$
* Option C: $P(Y > 2) > 0.5$
* Option D: $P(Y > 2) < 0.8$
```

### Question 10
```
Let's analyze each option:

Option A: To find the local minimum point, we need to find the critical points of f(x) by taking its derivative:

f'(x) = d/dx [(x - 1)^2(x - 4)] = 2(x - 1)(x - 4) + (x - 1)^2

Setting f'(x) = 0, we get:

2(x - 1)(x - 4) + (x - 1)^2 = 0
(x - 1)[2(x - 4) + (x - 1)] = 0
(x - 1)(2x - 7) = 0

This gives us critical points at x = 1 and x = 7/2. Now, we need to check the sign of f'(x) around these points to determine if they are local minima or maxima.

f'(x) > 0 when x < 1 or x > 7/2, and f'(x) < 0 when 1 < x < 7/2. Therefore, x = 1 is a local minimum point, but x = 3 is not. So, Option A is incorrect.

Option B: Let's analyze the inequality f(x) < f(x^2) when 0 < x < 1.

f(x) = (x - 1)^2(x - 4) < 0 when 0 < x < 1 (since x - 1 < 0 and x - 4 < 0)

f(x^2) = (x^2 - 1)^2(x^2 - 4) > 0 when 0 < x < 1 (since x^2 - 1 > 0 and x^2 - 4 < 0)

So, f(x) < f(x^2) when 0 < x < 1. Therefore, Option B is correct.

Option C: Let's analyze the inequality -4 < f(2x - 1) < 0 when 1 < x < 2.

f(2x - 1) = ((2x - 1) - 1)^2((2x - 1) - 4) = (2x - 2)^2(2x - 5)

When 1 < x < 2, we have 2 < 2x < 4, so 0 < 2x - 2 < 2 and -1 < 2x - 5 < 1.

(2x - 2)^2 > 0, and -1 < 2x - 5 < 1 implies -4 < (2x - 5) < 0.

Therefore, -4 < f(2x - 1) < 0 when 1 < x < 2. So, Option C is correct.

Option D: Let's analyze the inequality f(2 - x) > f(x) when -1 < x < 0.

f(2 - x) = ((2 - x) - 1)^2((2 - x) - 4) = (1 - x)^2(-2 - x)

f(x) = (x - 1)^2(x - 4)

When -1 < x < 0, we have 1 < 1 - x < 2 and -2 < -2 - x < -1.

(1 - x)^2 > 0, and -2 < -2 - x < -1 implies -4 < (1 - x)^2(-2 - x) < 0.

(x - 1)^2 > 0, and -1 < x - 4 < -4 implies -4 < (x - 1)^2(x - 4) < 0.

Since both f(2 - x) and f(x) are negative when -1 < x < 0, we need to compare their absolute values:

|(1 - x)^2(-2 - x)| > |(x - 1)^2(x - 4)| when -1 < x < 0

This inequality is true when -1 < x < 0. Therefore, Option D is correct.

So, the correct options are:

* Option B: When $0 < x < 1$, $f(x) < f(x^2)$
* Option C: When $1 < x < 2$, $-4 < f(2x - 1) < 0$
* Option D: When $-1 < x < 0$, $f(2 - x) > f(x)$
```

### Question 11
```
Let's break down the problem step by step!

Since the product of the distances from the point $O$ to $F(2, 0)$ and from $O$ to the line $x = a$ is equal to 4, we can write an equation:

$$|2-a|\cdot|2|=4$$

Since $a<0$, we have $|2-a|=2-a$ and $|2|=2$. So, the equation becomes:

$$2(2-a)=4$$

Solving for $a$, we get:

$$a=-2$$

So, Option A is correct.

Now, let's consider the shape of the curve $C$. Since the product of the distances from $O$ to $F(2, 0)$ and from $O$ to the line $x = a$ is equal to 4, we can write the equation of $C$ as:

$$y^2=(x+2)(2-x)$$

Simplifying the equation, we get:

$$y^2=-x^2-2x+4$$

Rearranging the equation, we get:

$$x^2+2x+y^2-4=0$$

This is an ellipse with center $(1, 0)$ and vertices at $(2, 0)$ and $(-2, 0)$. Since the point $(2\sqrt{2}, 0)$ lies outside the ellipse, Option B is incorrect.

The ellipse does not have a vertical asymptote at $x = 1$, so Option C is incorrect.

Finally, let's consider Option D. We can rewrite the equation of the ellipse as:

$$y^2=-x^2-2x+4$$

Rearranging the equation, we get:

$$y^2=-x(x+2)+4$$

Since $x>-2$, we have $x+2>0$. Therefore, $y^2\leq 4$, which implies:

$$y\leq\frac{4}{x+2}$$

So, Option D is correct.

In conclusion, the correct options are:

* Option A: $a = -2$
* Option D: when the point $(x_0, y_0)$ lies on $C$, then $y_0 \leq \frac{4}{x_0 + 2}$
```

## Fill-in-the-blank 
### Question 12
```
Let's break this problem down step by step!

Since the line passing through $F_2$ and parallel to the $y$-axis intersects $C$ at points $A$ and $B$, we can conclude that $F_2A = F_2B$. Let's call the distance $F_2A = F_2B = k$.

Now, we are given that $|F_1A| = 13$ and $|AB| = 10$. We can use the fact that $F_1A = F_1F_2 + F_2A$ to write:

$$13 = |F_1A| = |F_1F_2| + |F_2A| = |F_1F_2| + k$$

We know that $|F_1F_2| = 2ae$, where $e$ is the eccentricity of the hyperbola. So, we can rewrite the equation as:

$$13 = 2ae + k$$

Now, let's consider the point $B$. We have:

$$|F_1B| = |F_1A| - |AB| = 13 - 10 = 3$$

Using the same logic as before, we can write:

$$3 = |F_1B| = |F_1F_2| - |F_2B| = 2ae - k$$

Now we have two equations:

$$13 = 2ae + k$$
$$3 = 2ae - k$$

Adding these two equations, we get:

$$16 = 4ae \Rightarrow e = \frac{16}{4a} = \frac{4}{a}$$

So, the eccentricity of the hyperbola is $e = \frac{4}{a}$.

Note that we didn't need to find the values of $a$ and $b$ explicitly, as the problem only asked for the eccentricity $e$.
```

### Question 13
```
The derivative of $y=e^x+x$ is $y'=e^x+1$, so the slope of the tangent line at $(0,1)$ is $e^0+1=2$.  The derivative of $y=\ln(x+1)+a$ is $y'=\frac{1}{x+1}$, so the slope of the tangent line at $(0,a)$ is $\frac{1}{0+1}=1$.  Since these slopes must be equal, we have $2=1$, which is a contradiction.  Therefore, there is no such $a$.

However, if we assume that the point of tangency is not $(0,a)$, then we can solve for $a$.  Let the point of tangency be $(x_0,\ln(x_0+1)+a)$.  Then the slope of the tangent line is $\frac{1}{x_0+1}$.  Since we know that this slope is equal to $2$, we have $$\frac{1}{x_0+1}=2\Rightarrow x_0=\frac{1}{2}-1=-\frac{1}{2}.$$Then, since $y_0=\ln(x_0+1)+a$, we have $$1=\ln\left(\frac{1}{2}+1\right)+a=\ln\left(\frac{3}{2}\right)+a\Rightarrow a=1-\ln\left(\frac{3}{2}\right)=\boxed{1-\ln\left(\frac{3}{2}\right)}.$$
Final Answer: The final answer is 1-\ln\left(\frac{3}{2}\right). I hope it is correct.
```

### Question 14
```
Let's break down the possible outcomes and calculate the probability of A's total score being at least 2.

**Round 1:**
A wins with probability 2/4 (selecting 3, 5, or 7) and B wins with probability 2/4 (selecting 2 or 4).

**Round 2:**
Assuming A won in Round 1, A wins again with probability 2/3 (selecting 5 or 7) and B wins with probability 1/3 (selecting 2 or 4). If B won in Round 1, A wins with probability 3/3 (selecting 3, 5, or 7) and B wins with probability 0/3.

**Round 3:**
Assuming A won in Rounds 1 and 2, A wins again with probability 1/2 (selecting 7) and B wins with probability 1/2 (selecting 2, 4, or 6). If A won in Round 1 and B won in Round 2, A wins with probability 2/2 (selecting 5 or 7) and B wins with probability 0/2. If B won in Rounds 1 and 2, A wins with probability 3/3 (selecting 3, 5, or 7) and B wins with probability 0/3.

**Round 4:**
Assuming A won in Rounds 1, 2, and 3, A wins again with probability 1/1 (selecting 7) and B wins with probability 0/1. If A won in Rounds 1 and 2, and B won in Round 3, A wins with probability 1/1 (selecting 7) and B wins with probability 0/1. If A won in Round 1, and B won in Rounds 2 and 3, A wins with probability 2/2 (selecting 5 or 7) and B wins with probability 0/2. If B won in Rounds 1, 2, and 3, A wins with probability 3/3 (selecting 3, 5, or 7) and B wins with probability 0/3.

Now, let's calculate the probability of A's total score being at least 2:

* A wins all 4 rounds: (2/4) × (2/3) × (1/2) × (1/1) = 1/12
* A wins 3 rounds and loses 1 round: (2/4) × (2/3) × (1/2) × (0/1) + (2/4) × (1/3) × (2/2) × (1/1) + (2/4) × (1/3) × (0/2) × (2/2) = 1/6 + 1/6 + 0 = 1/3
* A wins 2 rounds and loses 2 rounds: (2/4) × (1/3) × (1/2) × (0/1) + (2/4) × (1/3) × (0/2) × (1/1) + (2/4) × (0/3) × (2/2) × (1/1) + (2/4) × (0/3) × (1/2) × (2/2) = 0 + 0 + 1/6 + 1/6 = 1/3

Adding up these probabilities, we get:

P(A's total score ≥ 2) = 1/12 + 1/3 + 1/3 = 11/12

So, the probability that A's total score is at least 2 is 11/12.
```
